Add LoVe06 homework

lean/LoVe/LoVe06_InductivePredicates_HomeworkSheet.lean
@@ -28,25 +28,33 @@ inductive Term : Type
 its argument is of the form `Term.lam …` and that returns `False` otherwise. -/
 
 -- enter your definition here
+
+inductive IsLam : Term → Prop where
+  | lam : ∀ (s : String) (t : Term), IsLam (Term.lam s t)
+
+/-
 def IsLam : Term -> Prop
   | .var _ => False
   | .lam _ _ => True
   | .app _ _ => False
+-/
 
 /- 1.2 (2 points). Validate your answer to question 1.1 by proving the following
 theorems: -/
 
 theorem IsLam_lam (s : String) (t : Term) :
-    IsLam (Term.lam s t) :=
-  sorry
+    IsLam (Term.lam s t) := by
+  apply IsLam.lam
 
 theorem not_IsLamVar (s : String) :
-    ¬ IsLam (Term.var s) :=
-  sorry
+    ¬ IsLam (Term.var s) := by
+  intro h
+  cases h
 
 theorem not_IsLam_app (t u : Term) :
-    ¬ IsLam (Term.app t u) :=
-  sorry
+    ¬ IsLam (Term.app t u) := by
+  intro h
+  cases h
 
 
 /- ## Question 2 (6 points): Transitive Closure
@@ -74,6 +82,11 @@ Define a predicate `TCV2` that embodies this alternative definition. -/
 
 -- enter your definition here
 
+inductive TCV2 {α : Type} (R : α → α → Prop) : α → α → Prop where
+  | base (a b : α)  : R a b → TCV2 R a b
+  | pets (a b c : α)  : TCV2 R a b → R b c → TCV2 R a c
+
+
 /- 2.2 (2 points). Yet another definition of the transitive closure `R⁺` would
 use the following symmetric rule instead of `(step)` or `(pets)`:
 
@@ -83,18 +96,30 @@ Define a predicate `TCV3` that embodies this alternative definition. -/
 
 -- TODO: enter your definition here
 inductive TCV3 {α : Type} (R : α → α → Prop) : α → α → Prop
+  | base (a b : α)  : R a b → TCV3 R a b
+  | trans (a b c : α)  : TCV3 R a b → TCV3 R b c → TCV3 R a c
 
 /- 2.3 (1 point). Prove that `(step)` also holds as a theorem about `TCV3`. -/
 
 theorem TCV3_step {α : Type} (R : α → α → Prop) (a b c : α) (rab : R a b)
       (tbc : TCV3 R b c) :
-    TCV3 R a c :=
-  sorry
+    TCV3 R a c := by
+  cases tbc with
+    | base b c hbc =>
+      exact TCV3.trans a b c (TCV3.base a b rab) (TCV3.base b c hbc)
+    -- b -> c via b -> x -> c
+    | trans b x c tbx txc =>
+      exact TCV3.trans a b c (TCV3.base a b rab) (TCV3.trans b x c tbx txc)
 
 /- 2.4 (1 point). Prove the following theorem by rule induction: -/
 
 theorem TCV1_pets {α : Type} (R : α → α → Prop) (c : α) :
-    ∀a b, TCV1 R a b → R b c → TCV1 R a c :=
-  sorry
+    ∀a b, TCV1 R a b → R b c → TCV1 R a c := by
+  intro a b tab rbc
+  induction tab with
+    | base a b rab =>
+      exact TCV1.step a b c rab (TCV1.base b c rbc)
+    | step a' x c' rax txc ihtxc =>
+      exact TCV1.step a' x c rax (ihtxc rbc)
 
 end LoVe
